extract/TyExtra.ml
@@ -1,0 +1,15 @@
+let oty_type = function Some ty -> ty | None -> raise UnexpectedProp
+
+
+let ts_tuple_ids = Hid.create 17
+
+let ts_tuple = Hint.memo 17 (fun n ->
+  let vl = ref [] in
+  for _i = 1 to n do vl := create_tvsymbol (id_fresh "a") :: !vl done;
+  let ts = create_tysymbol (id_fresh ("tuple" ^ string_of_int n)) !vl NoDef in
+  Hid.add ts_tuple_ids ts.ts_name n;
+  ts)
+
+let ty_tuple tyl = ty_app (ts_tuple (List.length tyl)) tyl
+
+let is_ts_tuple ts = ts_equal ts (ts_tuple (List.length ts.ts_args))
