src/util/StateMonad.v
@@ -1,46 +1,115 @@
-(*A mutable counter to register identifiers*)
+(*Several different state monads, which are extracted
+  to mutable references in OCaml*)
 Require CoqBigInt.
 Require Import Monad.
 
-(*We offer a restricted subset of the state monad interface
-  so that we can extract to OCaml mutable references soundly*)
-Definition ctr (a: Type) : Type := CoqBigInt.t -> CoqBigInt.t * a.
-
-(*Note: should not be used directly*)
-Definition ctr_get : ctr CoqBigInt.t := fun x => (x, x).
-
-Definition ctr_ret {a: Type} (x: a) : ctr a := fun s => (s, x).
-Definition ctr_bnd {a b: Type} (f: a -> ctr b) (x: ctr a) : ctr b :=
+(*Generalized state monad*)
+Definition state (s a: Type) : Type := s -> (s * a).
+Definition st_get {s: Type} : state s s := fun x => (x, x).
+Definition st_set {s: Type} (x: s) : state s unit := fun _ => (x, tt).
+Definition st_ret {s a: Type} (x: a) : state s a := fun s => (s, x).
+Definition st_bnd {s a b: Type} (f: a -> state s b) (m: state s a) : state s b :=
   fun i =>
-    let t := x i in
+    let t := m i in
     f (snd t) (fst t).
 
-(*Counter starts at 8- 1st 7 numbers are reserved*)
-Definition new_ctr : ctr unit := fun _ => (CoqBigInt.eight, tt).
-Definition incr : ctr unit := fun i => (CoqBigInt.succ i, tt).
+(*Combine multiple states*)
+(*NOTE: this is not a very good implementation, but
+  we don't want to do things generically, or else 
+  the OCaml code will have lots of Obj.magic*)
+(*TODO: generalize to (list Type)? This will give horrible
+  OCaml code most likely*)
+Definition state_multi (s1 s2 a: Type) : Type := state (s1 * s2) a.
+Definition st_get1 {s1 s2: Type} : state_multi s1 s2 s1 := fun x => (x, fst x).
+Definition st_get2 {s1 s2: Type} : state_multi s1 s2 s2 := fun x => (x, snd x).
+Definition st_set1 {s1 s2: Type} (x: s1) : state_multi s1 s2 unit :=
+  (fun y => ((x, snd y), tt)).
+Definition st_set2 {s1 s2: Type} (x: s2) : state_multi s1 s2 unit :=
+  (fun y => ((fst y, x), tt)).
+Definition st_multi_ret {s1 s2 a: Type} (x: a) : state_multi s1 s2 a := st_ret x.
+Definition st_multi_bnd {s1 s2 a b: Type} (f: a -> state_multi s1 s2 b)
+  (m: state_multi s1 s2 a) : state_multi s1 s2 b := st_bnd f m.
 
-(*TODO: remove*)
-From stdpp Require Import base.
-Global Instance ctr_ret': MRet ctr := @ctr_ret.
-Global Instance ctr_bnd': MBind ctr := @ctr_bnd.
+(*Combine state and error handling (monad transformer)*)
+Require Import ErrorMonad.
 
-(*A vile hack - for extraction, we need a type that does not
-  get erased when creating a counter*)
+(*We can't do monad transformers generically or else OCaml
+  code is bad. For now, we just combine state and error, and
+  the above lets us combine multiple states
+  (This is ExceptT on state monad)*)
+Definition exceptT (s a: Type) : Type :=
+  state s (errorM a).
+Definition exceptT_ret {s a: Type} (x: a) : exceptT s a :=
+  st_ret (ret x).
+Definition exceptT_bnd {s a b: Type} (f: a -> exceptT s b)
+  (m: exceptT s a) : exceptT s b :=
+  st_bnd (fun y =>
+    match y with
+    | Normal _ z => f z
+    | Error _ e => st_ret (Error _ e)
+    end
+  )m.
+Definition exceptT_lift {s a: Type} (x: state s a) : exceptT s a :=
+  st_bnd (fun s => st_ret (ret s)) x.
+Definition exceptT_lift2 {s a: Type} (x: errorM a) : exceptT s a :=
+  st_ret x.
+
+(*And now we include several kinds of state:*)
+(* 1. A mutable counter*)
+Definition ctr (a: Type) : Type := state CoqBigInt.t a.
+Definition ctr_get : ctr CoqBigInt.t := st_get.
+Definition ctr_ret {a: Type} (x: a) : ctr a := st_ret x.
+Definition ctr_bnd {a b: Type} (f: a -> ctr b) (m: ctr a) : ctr b := st_bnd f m.
+(*2 hacks: to create a new counter (which starts at the given value)
+  and a vile hack to ensure that we can set the type of the creation*)
+Definition new_ctr (i: CoqBigInt.t) : ctr unit := st_set i.
+(*TODO: see if we need this*)
+Definition incr : ctr unit := ctr_bnd 
+  (fun i => st_set (CoqBigInt.succ i)) ctr_get.
 Definition ctr_unit := ctr unit.
-
 Definition ctr_list {A: Type} (l: list (ctr A)) : ctr (list A) :=
   listM ctr_ret ctr_bnd l.
 
-(*Hash Consing*)
+(*2. Hash table*)
 Require Import Hashtbl.
-
-Section HashconsST.
+Section HashTbl.
+Definition hash_st (key a: Type) : Type := state (@hashtbl key) a.
 
 Context {key: Type} (hash: key -> CoqBigInt.t) 
   (eqb: key -> key -> bool).
 
-(*Because modules cannot be passed as parameters ugh*)
+Definition hash_get (a: Type) : hash_st key (@hashtbl key):= st_get.
+Definition hash_set (a: Type) (x: @hashtbl key) : hash_st key unit :=
+  st_set x.
+Definition hash_ret {a: Type} (x: a) : hash_st key a := st_ret x.
+Definition hash_bnd {a b: Type} (f: a -> hash_st key b) (m: hash_st key a) : hash_st key b :=
+  st_bnd f m.
+Definition new_hash : hash_st key unit := st_set create_hashtbl.
+Definition hash_unit := hash_st key unit.
+Definition hash_listM {A: Type} (l: list (hash_st key A))
+ := listM hash_ret hash_bnd l.
+
+(*3. Hash consing - combine 2 states*)
+Section HashconsST.
+
 Definition hashcons_st (a: Type) : Type :=
+  state_multi CoqBigInt.t (@hashtbl key) a.
+Definition hashcons_get_ctr : hashcons_st CoqBigInt.t :=
+  st_get1.
+Definition hashcons_get_hashtbl : hashcons_st (@hashtbl key) :=
+  st_get2.
+Definition hashcons_set_ctr (x: CoqBigInt.t) : hashcons_st unit :=
+  st_set1 x.
+Definition hashcons_set_hashtbl (h: @hashtbl key) : hashcons_st unit :=
+  st_set2 h.
+Definition hashcons_ret {a: Type} (d: a) : hashcons_st a :=
+  st_multi_ret d.
+Definition hashcons_bnd {A B: Type} (f: A -> hashcons_st B) 
+  (h: hashcons_st A) : hashcons_st B :=
+  st_multi_bnd f h.
+
+(*Because modules cannot be passed as parameters ugh*)
+(*Definition hashcons_st (a: Type) : Type :=
   (CoqBigInt.t * @hashtbl key) -> ((CoqBigInt.t * @hashtbl key) * a).
 Definition hashcons_incr : hashcons_st unit :=
   (fun x => (CoqBigInt.succ (fst x), snd x, tt)).
@@ -59,15 +128,22 @@ Definition hashcons_bnd {A B: Type} (f: A -> hashcons_st B)
   (h: hashcons_st A) : hashcons_st B :=
   fun x =>
     let t := h x in
-    f (snd t) (fst t).
+    f (snd t) (fst t).*)
 (*The hack again*)
 Definition hashcons_unit := hashcons_st unit.
 
 End HashconsST.
+End HashTbl.
 
 Definition hashcons_list {K A : Type} (l: list (@hashcons_st K A)) :
   @hashcons_st K (list A) :=
   listM hashcons_ret hashcons_bnd l.
+
+(*Combine error handling and hashcons*)
+(*TODO: combine with above*)
+(*Really, really want to do this generically*)
+(*Maybe I will try and hopefully get OCaml to be OK
+  with it*)
 
 
 (*Monad transformers (kind of)*)
