src/util/Exthtbl.v
@@ -1,0 +1,5 @@
+(*A (limited) implementation of hash tables*)
+Require Import Hashtbl.
+(*We do everything in a state monad. In OCaml, this will 
+  be a mutable reference storing a functional hash table*)
+
